src/tls/Crypto.Indexing.fst
@@ -37,29 +37,38 @@ record stack.
 (see mitls-fstar/.fstar/examples/low-level/crypto/Crypto.Indexing.fst)
 **)
 
-type id =
-  i:TLSInfo.id{~(PlaintextID? i) /\ TLSConstants.AEAD? (aeAlg_of_id i)}
+type aead_id (i:Idx.id) =
+  Idx.Derive? i /\
+  (let Idx.Derive _ _ ctx = i in
+  Idx.ExpandLog? ctx /\
+  ~(TLSInfo.LogInfo_CH? (Idx.ExpandLog?.info ctx)))
 
-let aeadAlg_of_id (i:id) =
-  let TLSConstants.AEAD a _ = aeAlg_of_id i in
-  match a with
+type id = i:Idx.id{aead_id i}
+
+let aeadAlg_of_id (i:id) : GTot aeadAlg =
+  let Idx.Derive _ _ (Idx.ExpandLog info _) = i in
+  match TLSInfo.logInfo_ae info with
   | CC.AES_128_GCM -> AES_128_GCM
   | CC.AES_256_GCM -> AES_256_GCM
   | CC.CHACHA20_POLY1305 -> CHACHA20_POLY1305
   | _ -> admit()
 
-let macAlg_of_id (i:id) =
-  match aeadAlg_of_id i with
+let macAlg_of_aeadAlg = function
   | AES_128_GCM       -> GHASH
   | AES_256_GCM       -> GHASH
   | CHACHA20_POLY1305 -> POLY1305
+  
+let macAlg_of_id (i:id) : GTot macAlg =
+  macAlg_of_aeadAlg (aeadAlg_of_id i)
 
-let cipherAlg_of_id (i:id) =
-  match aeadAlg_of_id i with
+let cipherAlg_of_aeadAlg = function
   | AES_128_GCM       -> AES128
   | AES_256_GCM       -> AES256
   | CHACHA20_POLY1305 -> CHACHA20
 
+let cipherAlg_of_id (i:id) : GTot cipherAlg =
+  cipherAlg_of_aeadAlg (aeadAlg_of_id i)
+  
 let aesImpl_of_id (i:id) = ValeAES
 
 let aeadAlg_cipherAlg (i:id) : Lemma
@@ -70,4 +79,12 @@ let aeadAlg_cipherAlg (i:id) : Lemma
      (aeadAlg_of_id i == CHACHA20_POLY1305 ==> cipherAlg_of_id i == CHACHA20)))
   = ()
 
-let testId (a:aeadAlg) = admit()
+private let name_convert = function
+  | AES_128_GCM -> CC.AES_128_GCM
+  | AES_256_GCM -> CC.AES_256_GCM
+  | CHACHA20_POLY1305 -> CC.CHACHA20_POLY1305
+
+let testId (a:aeadAlg) =
+  assume false;
+  Idx.Derive (Idx.Preshared Hashing.Spec.SHA256 0) "test"
+    (Idx.ExpandLog (LogInfo_CH0 ({li_ch0_cr = Bytes.create 32ul 0uy; li_ch0_ed_psk = Bytes.empty_bytes; li_ch0_ed_ae = (name_convert a); li_ch0_ed_hash = Hashing.Spec.SHA256})) Bytes.empty_bytes)
